proof/refine/X64/Refine.thy
@@ -11,7 +11,7 @@
 theory Refine
 imports
   KernelInit_R
-  DomainTime_R
+  ADT_H
   InitLemmas
   PageTableDuplicates
 begin
@@ -401,15 +401,22 @@ lemma ckernel_invs:
   apply (rule hoare_pre)
    apply (wp activate_invs' activate_sch_act schedule_sch
              schedule_sch_act_simple he_invs' schedule_invs'
+             hoare_drop_imp[where R="\<lambda>_. kernelExitAssertions"]
           | simp add: no_irq_getActiveIRQ)+
   done
 
-lemma doMachineOp_ct_running':
-  "\<lbrace>ct_running'\<rbrace> doMachineOp f \<lbrace>\<lambda>_. ct_running'\<rbrace>"
-  apply (simp add: ct_in_state'_def doMachineOp_def split_def)
-  apply wp
-  apply (simp add: pred_tcb_at'_def o_def)
-  done
+(* abstract and haskell have identical domain list fields *)
+abbreviation valid_domain_list' :: "'a kernel_state_scheme \<Rightarrow> bool" where
+  "valid_domain_list' \<equiv> \<lambda>s. valid_domain_list_2 (ksDomSchedule s)"
+
+lemmas valid_domain_list'_def = valid_domain_list_2_def
+
+defs kernelExitAssertions_def:
+  "kernelExitAssertions s \<equiv> 0 < ksDomainTime s \<and> valid_domain_list' s"
+
+lemma callKernel_domain_time_left:
+  "\<lbrace> \<top> \<rbrace> callKernel e \<lbrace>\<lambda>_ s. 0 < ksDomainTime s \<and> valid_domain_list' s \<rbrace>"
+  unfolding callKernel_def kernelExitAssertions_def by wpsimp
 
 lemma kernelEntry_invs':
   "\<lbrace> invs' and (\<lambda>s. e \<noteq> Interrupt \<longrightarrow> ct_running' s) and
@@ -424,7 +431,7 @@ lemma kernelEntry_invs':
   apply (wp ckernel_invs callKernel_domain_time_left
             threadSet_invs_trivial threadSet_ct_running' select_wp
             TcbAcc_R.dmo_invs' static_imp_wp
-            doMachineOp_ct_running' doMachineOp_sch_act_simple
+            doMachineOp_sch_act_simple
             callKernel_domain_time_left
          | clarsimp simp: user_memory_update_def no_irq_def tcb_at_invs'
                           valid_domain_list'_def)+
@@ -489,6 +496,9 @@ lemma device_update_invs':
                     gets_def get_def bind_def valid_def return_def)
    by (clarsimp simp: invs'_def valid_state'_def valid_irq_states'_def valid_machine_state'_def)
 
+crunches doMachineOp
+  for ksDomainTime[wp]: "\<lambda>s. P (ksDomainTime s)"
+
 lemma doUserOp_invs':
   "\<lbrace>invs' and ex_abs einvs and
     (\<lambda>s. ksSchedulerAction s = ResumeCurrentThread) and ct_running' and
@@ -498,7 +508,7 @@ lemma doUserOp_invs':
         (\<lambda>s. ksSchedulerAction s = ResumeCurrentThread) and ct_running' and
         (\<lambda>s. 0 < ksDomainTime s) and valid_domain_list'\<rbrace>"
   apply (simp add: doUserOp_def split_def ex_abs_def)
-  apply (wp device_update_invs' doMachineOp_ct_running' select_wp
+  apply (wp device_update_invs' select_wp
     | (wp (once) dmo_invs', wpsimp simp: no_irq_modify device_memory_update_def
                                        user_memory_update_def))+
   apply (clarsimp simp: user_memory_update_def simpler_modify_def
@@ -510,12 +520,21 @@ lemma doUserOp_invs':
 
 text \<open>The top-level correspondence\<close>
 
-lemma kernel_corres:
+lemma kernel_corres':
   "corres dc (einvs and (\<lambda>s. event \<noteq> Interrupt \<longrightarrow> ct_running s) and (ct_running or ct_idle)
                and (\<lambda>s. scheduler_action s = resume_cur_thread))
              (invs' and (\<lambda>s. event \<noteq> Interrupt \<longrightarrow> ct_running' s) and (ct_running' or ct_idle') and
               (\<lambda>s. ksSchedulerAction s = ResumeCurrentThread))
-             (call_kernel event) (callKernel event)"
+             (call_kernel event)
+             (do _ \<leftarrow> runExceptT $
+                      handleEvent event `~catchError~`
+                        (\<lambda>_. withoutPreemption $ do
+                               irq <- doMachineOp (getActiveIRQ True);
+                               when (isJust irq) $ handleInterrupt (fromJust irq)
+                             od);
+                 _ \<leftarrow> ThreadDecls_H.schedule;
+                 activateThread
+              od)"
   apply (simp add: call_kernel_def callKernel_def)
   apply (rule corres_guard_imp)
     apply (rule corres_split)
@@ -568,6 +587,33 @@ lemma device_mem_corres:
   by (clarsimp simp add: gets_def get_def return_def bind_def
                          invs_def invs'_def
                          corres_underlying_def device_mem_relation)
+
+lemma kernel_corres:
+  "corres dc (einvs and (\<lambda>s. event \<noteq> Interrupt \<longrightarrow> ct_running s) and (ct_running or ct_idle) and
+              (\<lambda>s. scheduler_action s = resume_cur_thread) and
+              (\<lambda>s. 0 < domain_time s \<and> valid_domain_list s))
+             (invs' and (\<lambda>s. event \<noteq> Interrupt \<longrightarrow> ct_running' s) and (ct_running' or ct_idle') and
+              (\<lambda>s. ksSchedulerAction s = ResumeCurrentThread) and
+              (\<lambda>s. vs_valid_duplicates' (ksPSpace s)))
+             (call_kernel event) (callKernel event)"
+  unfolding callKernel_def K_bind_def
+  apply (rule corres_guard_imp)
+    apply (rule corres_add_noop_lhs2)
+    apply (simp only: bind_assoc[symmetric])
+    apply (rule corres_split[where r'=dc and
+                                   R="\<lambda>_ s. 0 < domain_time s \<and> valid_domain_list s" and
+                                   R'="\<lambda>_. \<top>"])
+       apply (rule corres_bind_return2, rule corres_stateAssert_assume_stronger)
+        apply simp
+       apply (simp add: kernelExitAssertions_def state_relation_def)
+      apply (simp only: bind_assoc)
+      apply (rule kernel_corres')
+     apply (wp call_kernel_domain_time_inv_det_ext call_kernel_domain_list_inv_det_ext)
+    apply wp
+   apply clarsimp
+  apply clarsimp
+  done
+
 
 lemma entry_corres:
   "corres (=) (einvs and (\<lambda>s. event \<noteq> Interrupt \<longrightarrow> ct_running s) and
@@ -818,12 +864,11 @@ lemma ckernel_invariant:
      apply (rule valid_corres_combined[OF do_user_op_invs2 corres_guard_imp2[OF do_user_op_corres]])
       apply clarsimp
      apply (rule doUserOp_invs'[THEN hoare_weaken_pre])
-     apply (fastforce simp: ex_abs_def domain_time_rel_eq domain_list_rel_eq)
+     apply (fastforce simp: ex_abs_def)
     apply (clarsimp simp: invs_valid_objs' ex_abs_def, rule_tac x=s in exI,
             clarsimp simp: ct_running_related sched_act_rct_related)
    apply (clarsimp simp: ex_abs_def)
-   apply (fastforce simp: ex_abs_def ct_running_related sched_act_rct_related
-                          domain_time_rel_eq)
+   apply (fastforce simp: ex_abs_def ct_running_related sched_act_rct_related)
 
   apply (erule_tac P="a \<and> b \<and> c \<and> (\<exists>x. d x)" for a b c d in disjE)
    apply (clarsimp simp add: do_user_op_H_def monad_to_transition_def)
