proof/refine/X64/PageTableDuplicates.thy
@@ -10,10 +10,6 @@ begin
 
 context begin interpretation Arch . (*FIXME: arch_split*)
 
-
-(* we need the following lemma in Syscall_R *)
-crunch inv[wp]: getRegister "P"
-
 lemma doMachineOp_ksPSpace_inv[wp]:
   "\<lbrace>\<lambda>s. P (ksPSpace s)\<rbrace> doMachineOp f \<lbrace>\<lambda>ya s. P (ksPSpace s)\<rbrace>"
   by (simp add:doMachineOp_def split_def | wp)+
